proof/refine/ARM/VSpace_R.thy
@@ -2115,6 +2115,7 @@ proof -
        (\<forall>c. caps_of_state s p = Some c \<longrightarrow> P s \<and> Q s c)"
    by blast
   show ?thesis
+  apply add_cur_tcb'
   using assms
   apply (cases pgi)
      apply (rename_tac word cap prod sum)
@@ -2318,6 +2319,8 @@ proof -
     apply (auto simp: valid_page_inv_def invs_vspace_objs[simplified])[2]
   \<comment> \<open>PageGetAddr\<close>
   apply (clarsimp simp: perform_page_invocation_def performPageInvocation_def page_invocation_map_def fromPAddr_def)
+  apply (rule corres_stateAssert_add_assertion[rotated])
+    apply (clarsimp simp: cur_tcb'_asrt_def)
   apply (rule corres_guard_imp)
     apply (rule corres_split_deprecated[OF _ gct_corres])
       apply simp
@@ -2326,7 +2329,7 @@ proof -
         apply clarsimp
        apply (wp)+
    apply (clarsimp simp: tcb_at_invs)
-  apply (clarsimp simp: tcb_at_invs')
+  apply (clarsimp simp: cur_tcb'_def)
   done
 qed
 
@@ -2404,6 +2407,7 @@ lemma perform_page_table_corres:
           (perform_page_table_invocation pti)
           (performPageTableInvocation pti')"
   (is "?mp \<Longrightarrow> corres dc ?P ?P' ?f ?g")
+  apply add_cur_tcb'
   apply (simp add: perform_page_table_invocation_def performPageTableInvocation_def)
   apply (cases pti)
    apply (clarsimp simp: page_table_invocation_map_def)
@@ -2541,7 +2545,7 @@ lemma storeHWASID_invs:
    apply fastforce
   apply (simp add: storeHWASID_def)
   apply (wp findPDForASIDAssert_pd_at_wp)
-  apply (clarsimp simp: invs'_def valid_state'_def valid_arch_state'_def valid_dom_schedule'_def
+  apply (clarsimp simp: invs'_def valid_arch_state'_def valid_dom_schedule'_def
              valid_global_refs'_def global_refs'_def valid_machine_state'_def
              ct_not_inQ_def ct_idle_or_in_cur_domain'_def tcb_in_cur_domain'_def)
   done
@@ -2555,7 +2559,7 @@ lemma findFreeHWASID_invs:
                    doMachineOp_def split_def
               cong: option.case_cong)
   apply (wp findPDForASIDAssert_pd_at_wp | wpc)+
-  apply (clarsimp simp: invs'_def valid_state'_def valid_arch_state'_def
+  apply (clarsimp simp: invs'_def valid_arch_state'_def
              valid_global_refs'_def global_refs'_def valid_machine_state'_def
              ct_not_inQ_def valid_dom_schedule'_def
            split del: if_split)
@@ -2710,7 +2714,7 @@ lemma storePDE_invs[wp]:
           and (\<lambda>s. valid_pde_mapping' (p && mask pdBits) pde)\<rbrace>
       storePDE p pde
    \<lbrace>\<lambda>_. invs'\<rbrace>"
-  apply (simp add: invs'_def valid_state'_def valid_pspace'_def valid_dom_schedule'_def)
+  apply (simp add: invs'_def valid_pspace'_def valid_dom_schedule'_def)
   apply (rule hoare_pre)
    apply (wp sch_act_wf_lift valid_global_refs_lift'
              irqs_masked_lift
@@ -2752,7 +2756,7 @@ lemma storePTE_pde_mappings'[wp]:
 
 lemma storePTE_invs [wp]:
   "\<lbrace>invs' and valid_pte' pte\<rbrace> storePTE p pte \<lbrace>\<lambda>_. invs'\<rbrace>"
-  apply (simp add: invs'_def valid_state'_def valid_pspace'_def valid_dom_schedule'_def)
+  apply (simp add: invs'_def valid_pspace'_def valid_dom_schedule'_def)
   apply (rule hoare_pre)
    apply (wp sch_act_wf_lift valid_global_refs_lift' irqs_masked_lift
              valid_arch_state_lift' valid_irq_node_lift
@@ -2797,7 +2801,7 @@ lemma setObject_asidpool_mappings'[wp]:
 
 lemma setASIDPool_invs [wp]:
   "\<lbrace>invs' and valid_asid_pool' ap\<rbrace> setObject p (ap::asidpool) \<lbrace>\<lambda>_. invs'\<rbrace>"
-  apply (simp add: invs'_def valid_state'_def valid_pspace'_def valid_dom_schedule'_def)
+  apply (simp add: invs'_def valid_pspace'_def valid_dom_schedule'_def)
   apply (rule hoare_pre)
    apply (wp sch_act_wf_lift valid_global_refs_lift' irqs_masked_lift
              valid_arch_state_lift' valid_irq_node_lift
@@ -2959,8 +2963,9 @@ lemma perform_pt_invs [wp]:
   "\<lbrace>invs' and valid_page_inv' pt\<rbrace> performPageInvocation pt \<lbrace>\<lambda>_. invs'\<rbrace>"
   apply (simp add: performPageInvocation_def)
   apply (cases pt)
-     apply clarsimp
-     apply ((wp dmo_invs' hoare_vcg_all_lift setVMRootForFlush_invs' | simp add: tcb_at_invs')+)[2]
+     apply (clarsimp simp: cur_tcb'_asrt_def)
+     apply (rule hoare_seq_ext[OF _ stateAssert_sp])
+     apply ((wp dmo_invs' hoare_vcg_all_lift setVMRootForFlush_invs' | simp add: cur_tcb'_def)+)[2]
        apply (rule hoare_pre_imp[of _ \<top>], assumption)
        apply (clarsimp simp: valid_def
                              disj_commute[of "pointerInUserData p s" for p s])
